Clean file, but still failing

src/substitutions.v
@@ -68,10 +68,9 @@ Section Substitutions.
 
   Open Scope type_scope.
 
-(* Let's do it with preconditions for now *)
-(* Context `{configPrecondition : config.Precondition}. *)
-Local Instance havePrecondition : config.Precondition :=
-  {| config.flagPrecondition := config.Yes |}.
+Context `{configPrecondition : config.Precondition}.
+(* Local Instance havePrecondition : config.Precondition := *)
+(*   {| config.flagPrecondition := config.Yes |}. *)
 Context `{configReflection : config.Reflection}.
 Context `{configBinaryProdType : config.BinaryProdType}.
 Context `{configProdEta : config.ProdEta}.
@@ -84,94 +83,6 @@ Context `{configUnitType : config.UnitType}.
 Context `{configBoolType : config.BoolType}.
 Context `{configProdType : config.ProdType}.
 Context `{configSyntax : syntax.Syntax}.
-
-Fixpoint issubst_rec (σ : substitution) (Γ Δ : context) (hΔ : isctx Δ) : Type.
-  destruct hΔ as [| Δ A hΔ hA].
-  - exact Datatypes.unit.
-  - doConfig.
-    simple refine (_ * _).
-    + exact (issubst_rec σ↑ Γ Δ hΔ).
-    + exact (isterm Γ (var 0)[σ] A[σ↑]).
-Defined.
-
-Definition issubst σ Γ Δ := { h : isctx Δ & issubst_rec σ Γ Δ h }.
-
-Lemma SubstNil :
-  forall {σ Γ},
-    isctx Γ ->
-    issubst σ Γ ctxempty.
-Proof.
-  intros σ Γ hΓ.
-  exists CtxEmpty. exact tt.
-Defined.
-
-Lemma SubstCons :
-  forall {σ Γ Δ A},
-    isctx Γ ->
-    isctx Δ ->
-    istype Δ A ->
-    issubst (σ↑) Γ Δ ->
-    isterm Γ (var 0)[σ] A[σ↑] ->
-    issubst σ Γ (ctxextend Δ A).
-Proof.
-  intros σ Γ Δ A hΓ _ hA [hΔ hσ] hv.
-  unshelve eexists.
-  - now capply CtxExtend.
-  - cbn. split.
-    + assumption.
-    + assumption.
-Defined.
-
-Lemma issubst_ext :
-  forall {Γ Δ},
-    isctx Γ ->
-    isctx Δ ->
-    forall {σ ρ},
-      σ ~ ρ ->
-      issubst σ Γ Δ ->
-      issubst ρ Γ Δ.
-Proof.
-  intros Γ Δ hΓ hΔ.
-  induction hΔ as [| Δ B hΔ ih hB] ; intros σ ρ h [hΔB hσ].
-  - now exists CtxEmpty.
-  - doConfig.
-    specialize (ih (σ↑) (ρ↑)).
-    assert (hh : σ ↑ ~ ρ ↑).
-    { intro n. rewrite_substs. apply h. }
-    specialize (ih hh).
-    assert (hσ' : issubst σ↑ Γ Δ).
-    {
-
- (* exists hΔB. inversion hΔB as [| Δ' B' hΔ' hB']. *)
- (*    + (* Impossible case but true. *) *)
- (*      subst. easy. *)
- (*    + cbn. destruct hσ as [hσ hv]. *)
- (*      split. *)
- (*      * specialize (ih (σ↑) (ρ↑)). *)
- (*        assert (hh : σ ↑ ~ ρ ↑). *)
- (*        { intro n. rewrite_substs. apply h. } *)
- (*        specialize (ih hh). *)
- (*        assert (hσ' : issubst σ↑ Γ Δ). *)
- (*        { *)
-Abort.
-(* Working by induction on the derivation is really annoying when what
-   we really want is to work by induction on contexts.
- *)
-
-
-Lemma SubstWeak :
-  forall {Γ A},
-    isctx Γ ->
-    istype Γ A ->
-    issubst sbweak (ctxextend Γ A) Γ.
-Proof.
-  intros Γ A hΓ hA.
-  exists hΓ. induction hΓ as [| Δ B hΔ ih hB].
-  - exact tt.
-  - split.
-    +
-Abort.
-
 
 (* A substitution is well-formed if it is well-formed on variables.
    The action on types and terms is derived from it.
@@ -190,81 +101,22 @@ Inductive issubst : forall (σ : substitution) (Γ : context), context -> Type :
       issubst (σ↑) Γ Δ ->
       isterm Γ (var 0)[σ] A[σ↑] ->
       issubst σ Γ (ctxextend Δ A)
-
-| SubstWeak :
-    forall {Γ A},
-      isctx Γ ->
-      istype Γ A ->
-      issubst sbweak (ctxextend Γ A) Γ
 .
 
-Lemma issubst_ext :
-  forall {Γ Δ},
-    isctx Γ ->
-    isctx Δ ->
-    forall {σ ρ},
-      σ ~ ρ ->
-      issubst σ Γ Δ ->
-      issubst ρ Γ Δ.
-Proof.
-  intros Γ Δ hΓ hΔ.
-  induction hΔ ; intros σ ρ h hσ.
-  - apply SubstNil. assumption.
-  - rename G into Δ.
-    inversion hσ.
-    + apply SubstNil. assumption.
-    + doConfig.
-      assert (Δ0 = Δ).
-      { eapply ctxextend_inj. apply H2. }
-      assert (A0 = A).
-      { eapply ctxextend_inj. apply H2. }
-      subst.
-      apply SubstCons.
-      * assumption.
-      * assumption.
-      * assumption.
-      * apply X with (σ := σ ↑).
-        -- intro n. rewrite_substs. apply h.
-        -- assumption.
-      * (* Some setoid rewrite might help me? *)
-        (* It is true, but I'm lazy for now. *)
-        admit.
-    + subst. rename A0 into B.
-Abort. (* Maybe no longer necessary. *)
+Class SubstitutionProperties := {
+  SubstId   : forall {Γ}, isctx Γ -> issubst sbid Γ Γ;
+  SubstWeak : forall {Γ A}, isctx Γ -> istype Γ A -> issubst sbweak (Γ,A) Γ;
+  issubst_ext :
+    forall {Γ Δ},
+      isctx Γ ->
+      isctx Δ ->
+      forall {σ ρ},
+        σ ~ ρ ->
+        issubst σ Γ Δ ->
+        issubst ρ Γ Δ
+}.
 
-Fact eqDropCons : forall {u σ}, (u ⋅ σ) ↑ ~ σ.
-Proof.
-  intros u σ n.
-  now rewrite_substs.
-Defined.
-
-Lemma SubstCons' :
-  forall {Γ Δ A u σ},
-    isctx Γ ->
-    isctx Δ ->
-    issubst σ Γ Δ ->
-    istype Δ A ->
-    isterm Γ u A[σ] ->
-    issubst (u ⋅ σ) Γ (ctxextend Δ A).
-Proof.
-  intros Γ Δ A u σ hΓ hΔ hσ hA hu.
-  apply SubstCons.
-  - assumption.
-  - (* apply issubst_ext with (σ0 := σ). *)
-(*     + assumption. *)
-(*     + assumption. *)
-(*     + (* symmetry. *) *)
-(*       intro n. symmetry. *)
-(*       apply eqDropCons. *)
-(*     + assumption. *)
-(*   - rewrite_substs. *)
-(*     (* Some setoid rewrite would help us. *)
-(*        We'll only deal with those once we are convinced we're on the right *)
-(*        tracks. *)
-(*      *) *)
-(*     admit. *)
-(* Admitted. *)
-Abort.
+Context {substProp : SubstitutionProperties}.
 
 Lemma SubstCtxConv :
   forall {σ Γ Δ Δ'},
@@ -272,78 +124,14 @@ Lemma SubstCtxConv :
     issubst σ Γ Δ ->
     issubst σ Γ Δ'.
 Proof.
-  intros σ Γ Δ Δ' h1 h2.
-  induction h2.
+  intros σ Γ Δ Δ' eq hσ.
+  induction hσ.
   -
+Abort.
 
-  ceapply TermCtxConv.
-  - apply h2.
-    ceapply TermCtxConv.
-    + eassumption.
-    + assumption.
-    + admit. (* Need precondition *)
-    + admit. (* Need precondition *)
-    + admit. (* Need precondition *)
-  - capply CtxRefl. admit. (* Need precondition *)
-  - admit. (* Need precondition *)
-  - admit. (* Need precondition *)
-  - admit. (* Precondition in the definition of issubst? *)
-Admitted.
-
-(* We show applying substitutions preserves typing. *)
-Lemma TySubst :
-  forall {Δ A},
-    istype Δ A ->
-    forall {Γ σ},
-      issubst σ Γ Δ ->
-      istype Γ A[σ].
-Proof.
-  intros Δ A hA.
-  induction hA ; intros Γ σ hσ.
-
-  (* TyCtxConv *)
-  - { apply IHhA. ceapply SubstCtxConv.
-      - eassumption.
-      - assumption.
-    }
-
-  (* TyProd *)
-  - { rewrite_substs.
-      capply TyProd.
-      - apply IHhA. (* apply SubstCons. *)
-        (* We do it by hand, hopefully understanding who is SubstCons *)
-        intros [| n] C h.
-        + rewrite_substs.
-          (* Here we would need some kind of inversion AND induction
-             hypothesis. *)
-          admit.
-        + rewrite_substs. admit.
-      - apply X. assumption.
-      - admit. (* ok *)
-    }
-
-  (* TyId *)
-  - admit.
-
-  (* TyEmpty *)
-  - admit.
-
-  (* TyUnit *)
-  - admit.
-
-  (* TyBool *)
-  - admit.
-
-  (* TyBinaryProd *)
-  - admit.
-
-  (* TyUni *)
-  - admit.
-
-  (* TyEl *)
-  - admit.
-Admitted.
-
+(* Even when you admit most of the work is done, it still seems that
+   there are representation problems.
+ *)
 
 
 End Substitutions.
